\section*{Problem 2}
%%%%% PROBLEM STATEMENT %%%%%%%%%%%%%%%%%%%%%%%%%%%%%%%%%%%%%%%%%
\begin{myanswerbox}
While proving the Hoeffding inequality, we said that two probabilities,
\[
    \prob{\frac{1}{n} \sum_{i=1}^{n} X_i - \mu \geq t }
\]
and
\[ 
    \prob{\frac{1}{n} \sum_{i=1}^{n} X_i - \mu \leq -t },
\]
can be bounded in the same way and did the derivation only for the former probability. Show that the latter probability is indeed bounded by the same quantity.
\end{myanswerbox}
%%%%% QUESTION SEPARATOR %%%%%%%%%%%%%%%%%%%%%%%%%%%%%%%%%%%%%%%%
%%%%% Answer %%%%%

\begin{proof}
    Lets define $Z_i = X_i - \mu, \forall i = 1, 2, \dots, n$. Then, we have:
    
    \begin{align*}
    \bar{Z}_n = \frac{1}{n} \sum_{i=1}^n Z_i = \bar{X}_n - \mu
    \end{align*}
    
    and,
    
    \begin{align*}
    |Z_i| \leq a, \forall i = 1, 2, \dots , n
    \end{align*}
    
    then, whe can rewrite the former probability as:
    
    \begin{align*}
    \prob{\frac{1}{n} \sum_{i=1}^{n} X_i - \mu \leq -t } = \prob{\bar{Z}_n \geq -t}
    \end{align*}
    
    Expanding the average $\bar{Z}_n$:
    \begin{align*}
    \prob{\bar{Z}_n \geq -t} = \prob{\sum_{i=1}^n Z_i \leq -nt}
    \end{align*}
    
    for any $\lambda > 0$, we have \footnote{Given that $f(x) = \lambda x$ is a monotonically increasing function when $\lambda > 0$}:
    
    \begin{align*}
    \prob{\bar{Z}_n \geq -t} = 
    \prob{\lambda \sum_{i=1}^n Z_i \leq -\lambda nt}\\
    \end{align*}
    
    and, by Markov's inequality:
    
    \begin{align*}
    \prob{\lambda \sum_{i=1}^n Z_i \leq -\lambda nt} 
    \leq
    \frac{\E{\exp(\lambda \sum_{i=1}^n Z_i)}}{\exp(-\lambda nt)}
    \end{align*}
    
    since $Z_i$ are independent and identically distributed, we can write:
    
    \begin{align*}
    \frac{\E{\exp(\lambda \sum_{i=1}^n Z_i)}}{\exp(-\lambda nt)} 
    &=
    \frac{\prod_{i=1}^n \E{\exp(-\lambda Z_i)}}{\exp(-\lambda nt)}\\
    %%%%%
    &=
    \frac{\prod_{i=1}^n \exp(-1)\E{\exp(\lambda Z_i)}}{\exp(-\lambda nt)}\\
    %%%%%
    &=
        \frac{\prod_{i=1}^n \E{\exp(\lambda Z_i)}}{\exp(\lambda nt)} 
    \end{align*}
    
    Applying the Hoeffding's lemma \footnote{
        If $X$ is a random variable such that $X \leq a$, then for any $\lambda > 0$, we have:
        \begin{align*}
        \E{\exp(\lambda X)} 
        \leq
        \exp\left(\frac{\lambda^2a^2}{2}\right)
        \end{align*}
    } to the above expression, we have:
    
    \begin{align*}
    \frac{\prod_{i=1}^n \E{\exp(\lambda Z_i)}}{\exp(\lambda nt)} 
    &\leq
    \frac{\prod_{i = 1}^n \exp\left(\frac{\lambda^2a^2}{2}\right)}{\exp(\lambda nt)}\\
    %%%%%
    &\leq
    \frac{\exp\left(\frac{n\lambda^2a^2}{2}\right)}{\exp(\lambda nt)}\\
    %%%%%
   &\leq
    \exp\left(\frac{n\lambda^2a^2}{2} - \lambda nt \right)\\
    \end{align*}
    
    Because the above inequality holds for any $\lambda > 0$, we can optimize the right-hand side with respect to $\lambda$.
    
    \begin{align*}
    \lambda^* = \argmin_{\lambda > 0} \left\{ \frac{n\lambda^2a^2}{2} - \lambda nt \right\}
    \end{align*}
    
    Calculating the F.O.C. with respect to $\lambda$, we get:
    
    \begin{align*}
    n a^2 \lambda^* - nt = 0 \Rightarrow \lambda^* = \frac{t}{a^2}
    \end{align*}
    
    Substituting $\lambda^*$ back into the inequality:
    
    \begin{align*}
    \prob{\bar{Z}_n \geq -t} &\leq
        \exp\left(\frac{n\left(\frac{t}{a^2}\right)^2a^2}{2} - \frac{t}{a^2} n t \right)\\
    %%%%%
    &\leq
        \exp\left(\frac{nt^2}{2a^2} - \frac{nt^2}{a^2} \right)\\
    %%%%%
    &\leq
        \exp\left(-\frac{nt^2}{2a^2} \right)\\
    \end{align*}
    
    replacing $\bar{Z}_n$ by $\bar{X}_n - \mu$:
    
    \begin{align*}
    \prob{|\bar{X}_n - \mu| \geq t} \leq \exp\left(-\frac{nt^2}{2 a^2}\right)
    \end{align*}
    
    \end{proof}